fin

CRDT/ORSet3.thy
@@ -15,12 +15,12 @@ imports
   Network
 begin
 
-datatype ('id, 'a) operation = Add "'id" "'a" | Rem "'id set" "'a" | Append "'id" "'a" | Expunge "'a" "'id" "'id"
+datatype ('id, 'a) operation = Add "'id" "'a" | Rem "'id set" "'a" | Append "'id" "'a" | Expunge "'a" "'id" "'id" | Store "'a" "'id" "'id"
 
 type_synonym ('id, 'a) state = "'a \<Rightarrow> ('id set \<times> 'id set)"
 
 definition op_elem :: "('id, 'a) operation \<Rightarrow> 'a" where
-  "op_elem oper \<equiv> case oper of Add i e \<Rightarrow> e | Rem is e \<Rightarrow> e | Append i e \<Rightarrow> e | Expunge e mo i \<Rightarrow> e"
+  "op_elem oper \<equiv> case oper of Add i e \<Rightarrow> e | Rem is e \<Rightarrow> e | Append i e \<Rightarrow> e | Expunge e mo i \<Rightarrow> e | Store e mo i \<Rightarrow> e"
 
 definition interpret_op :: "('id, 'a) operation \<Rightarrow> ('id, 'a) state \<rightharpoonup> ('id, 'a) state" ("\<langle>_\<rangle>" [0] 1000) where
   "interpret_op oper state \<equiv>
@@ -30,7 +30,8 @@ definition interpret_op :: "('id, 'a) operation \<Rightarrow> ('id, 'a) state \<
 				   Add i e \<Rightarrow> (metadata \<union> {i}, files) |
 					 Rem is e \<Rightarrow> (metadata - is, files - is) |
 					 Append i e \<Rightarrow> (metadata, files \<union> {i}) |
-				   Expunge e mo i \<Rightarrow> (metadata \<union> {i}, files - {mo})
+				   Expunge e mo i \<Rightarrow> (metadata \<union> {i}, files - {mo}) |
+					 Store e mo i \<Rightarrow> (metadata, insert i (files - {mo}))
      in  Some (state ((op_elem oper) := after))"
   
 definition valid_behaviours :: "('id, 'a) state \<Rightarrow> 'id \<times> ('id, 'a) operation \<Rightarrow> bool" where
@@ -39,7 +40,8 @@ definition valid_behaviours :: "('id, 'a) state \<Rightarrow> 'id \<times> ('id,
        (i, Add j  e) \<Rightarrow> i = j |
        (i, Rem is e) \<Rightarrow> is = fst (state e) \<union> snd (state e) |
 			 (i, Append j e) \<Rightarrow> i = j |
-			 (i, Expunge e mo j) \<Rightarrow> i = j \<and> mo \<in> snd (state e)"
+			 (i, Expunge e mo j) \<Rightarrow> i = j \<and> mo \<in> snd (state e) |
+		   (i, Store e mo j) \<Rightarrow> i = j \<and> mo \<in> snd (state e)"
 
 locale orset = network_with_constrained_ops _ interpret_op "\<lambda>x. ({},{})" valid_behaviours
 
@@ -59,6 +61,10 @@ lemma (in orset) add_append_commute:
 lemma (in orset) add_expunge_commute:
   shows "\<langle>Add i1 e1\<rangle> \<rhd> \<langle>Expunge e2 mo i2\<rangle> = \<langle>Expunge e2 mo i2\<rangle> \<rhd> \<langle>Add i1 e1\<rangle>"
   by(auto simp add: interpret_op_def op_elem_def kleisli_def, fastforce)
+  	
+lemma (in orset) add_store_commute:
+  shows "\<langle>Add i1 e1\<rangle> \<rhd> \<langle>Store e2 mo i2\<rangle> = \<langle>Store e2 mo i2\<rangle> \<rhd> \<langle>Add i1 e1\<rangle>"
+  by(auto simp add: interpret_op_def op_elem_def kleisli_def, fastforce)
 
 lemma (in orset) rem_rem_commute:
   shows "\<langle>Rem i1 e1\<rangle> \<rhd> \<langle>Rem i2 e2\<rangle> = \<langle>Rem i2 e2\<rangle> \<rhd> \<langle>Rem i1 e1\<rangle>"
@@ -74,6 +80,11 @@ lemma (in orset) rem_expunge_commute:
   shows "\<langle>Rem is e1\<rangle> \<rhd> \<langle>Expunge e2 mo i\<rangle> = \<langle>Expunge e2 mo i\<rangle> \<rhd> \<langle>Rem is e1\<rangle>"
   using assms by(auto simp add: interpret_op_def kleisli_def op_elem_def, fastforce)
   	
+lemma (in orset) rem_store_commute:
+	assumes "i \<notin> is"
+  shows "\<langle>Rem is e1\<rangle> \<rhd> \<langle>Store e2 mo i\<rangle> = \<langle>Store e2 mo i\<rangle> \<rhd> \<langle>Rem is e1\<rangle>"
+  using assms by(auto simp add: interpret_op_def kleisli_def op_elem_def, fastforce)
+  	
 lemma (in orset) append_append_commute:
   shows "\<langle>Append i1 e1\<rangle> \<rhd> \<langle>Append i2 e2\<rangle> = \<langle>Append i2 e2\<rangle> \<rhd> \<langle>Append i1 e1\<rangle>"
   by(auto simp add: interpret_op_def op_elem_def kleisli_def, fastforce)
@@ -86,14 +97,40 @@ proof
 	show "(\<langle>Append i1 e1\<rangle> \<rhd> \<langle>Expunge e2 mo i2\<rangle>) x = (\<langle>Expunge e2 mo i2\<rangle> \<rhd> \<langle>Append i1 e1\<rangle>) x"
 		using assms by(auto simp add: interpret_op_def kleisli_def op_elem_def)
 qed
+	
+lemma (in orset) append_store_commute:
+  assumes "i1 \<noteq> mo"
+  shows "(\<langle>Append i1 e1\<rangle> \<rhd> \<langle>Store e2 mo i2\<rangle>) = (\<langle>Store e2 mo i2\<rangle> \<rhd> \<langle>Append i1 e1\<rangle>)"
+proof
+	fix x
+	show "(\<langle>Append i1 e1\<rangle> \<rhd> \<langle>Store e2 mo i2\<rangle>) x = (\<langle>Store e2 mo i2\<rangle> \<rhd> \<langle>Append i1 e1\<rangle>) x"
+		using assms by(auto simp add: interpret_op_def kleisli_def op_elem_def)
+qed
 
-  	
 lemma (in orset) expunge_expunge_commute:
   shows "(\<langle>Expunge e1 mo1 i1\<rangle> \<rhd> \<langle>Expunge e2 mo2 i2\<rangle>) = (\<langle>Expunge e2 mo2 i2\<rangle> \<rhd> \<langle>Expunge e1 mo1 i1\<rangle>)"
 proof
 	fix x
 	show "(\<langle>Expunge e1 mo1 i1\<rangle> \<rhd> \<langle>Expunge e2 mo2 i2\<rangle>) x = (\<langle>Expunge e2 mo2 i2\<rangle> \<rhd> \<langle>Expunge e1 mo1 i1\<rangle>) x"
-  by(auto simp add: interpret_op_def kleisli_def op_elem_def) qed
+		by(auto simp add: interpret_op_def kleisli_def op_elem_def) qed
+	
+lemma  expunge_store_commute:
+	assumes "i1 \<noteq> mo2" and "i2 \<noteq> mo1"
+  shows "(\<langle>Expunge e1 mo1 i1\<rangle> \<rhd> \<langle>Store e2 mo2 i2\<rangle>) = (\<langle>Store e2 mo2 i2\<rangle> \<rhd> \<langle>Expunge e1 mo1 i1\<rangle>)"
+proof
+	fix x
+	show "(\<langle>Expunge e1 mo1 i1\<rangle> \<rhd> \<langle>Store e2 mo2 i2\<rangle>) x = (\<langle>Store e2 mo2 i2\<rangle> \<rhd> \<langle>Expunge e1 mo1 i1\<rangle>) x"
+		unfolding  interpret_op_def kleisli_def op_elem_def using assms(2) by (simp, fastforce)
+qed
+	
+lemma (in orset) store_store_commute:
+	assumes "i1 \<noteq> mo2" and "i2 \<noteq> mo1"
+  shows "(\<langle>Store e1 mo1 i1\<rangle> \<rhd> \<langle>Store e2 mo2 i2\<rangle>) = (\<langle>Store e2 mo2 i2\<rangle> \<rhd> \<langle>Store e1 mo1 i1\<rangle>)"
+proof
+	fix x
+	show "(\<langle>Store e1 mo1 i1\<rangle> \<rhd> \<langle>Store e2 mo2 i2\<rangle>) x = (\<langle>Store e2 mo2 i2\<rangle> \<rhd> \<langle>Store e1 mo1 i1\<rangle>) x"
+		unfolding  interpret_op_def kleisli_def op_elem_def using assms by (simp, fastforce)
+qed
 
 lemma (in orset) apply_operations_never_fails:
   assumes "xs prefix of i"
@@ -142,6 +179,17 @@ proof -
   thus ?thesis
     by(simp add: valid_behaviours_def)
 qed
+	
+lemma (in orset) store_id_valid:
+  assumes "xs prefix of j"
+    and "Deliver (i1, Store e mo i2) \<in> set xs"
+  shows "i1 = i2"
+proof -
+  have "\<exists>s. valid_behaviours s (i1, Store e mo i2)"
+    using assms deliver_in_prefix_is_valid by blast
+  thus ?thesis
+    by(simp add: valid_behaviours_def)
+qed
 
 definition (in orset) added_ids :: "('id \<times> ('id, 'b) operation) event list \<Rightarrow> 'b \<Rightarrow> 'id list" where
   "added_ids es p \<equiv> List.map_filter (\<lambda>x. case x of 
@@ -152,6 +200,7 @@ definition (in orset) added_ids :: "('id \<times> ('id, 'b) operation) event lis
 definition (in orset) added_files :: "('id \<times> ('id, 'b) operation) event list \<Rightarrow> 'b \<Rightarrow> 'id list" where
     "added_files es p \<equiv> List.map_filter (\<lambda>x. case x of 
 		Deliver (i, Append j e) \<Rightarrow> if e = p then Some j else None |
+    Deliver (i, Store e mo j) \<Rightarrow> if e = p then Some j else None |
 		_ \<Rightarrow> None) es"
 		
 -- {* added files simplifier *}
@@ -187,6 +236,15 @@ lemma (in orset) added_files_Deliver_Append_diff_collapse [simp]:
 lemma (in orset) added_files_Deliver_Append_same_collapse [simp]:
   shows "added_files ([Deliver (i, Append j e)]) e = [j]"
   by (auto simp: added_files_def map_filter_append map_filter_def)
+  	
+lemma (in orset) added_files_Deliver_Store_diff_collapse [simp]:
+  shows "e \<noteq> e' \<Longrightarrow> added_files ([Deliver (i, Store e mo j)]) e' = []"
+  by (auto simp: added_files_def map_filter_append map_filter_def)
+    
+lemma (in orset) added_files_Deliver_Store_same_collapse [simp]:
+  shows "added_files ([Deliver (i, Store e mo j)]) e = [j]"
+  by (auto simp: added_files_def map_filter_append map_filter_def)
+  	
  
 -- {* added ids simplifier *}
   
@@ -209,6 +267,10 @@ lemma (in orset) added_ids_Deliver_Rem_collapse [simp]:
 lemma (in orset) added_ids_Deliver_Append_collapse [simp]:
   shows "added_ids ([Deliver (i, Append j e)]) e' = []"
   by (auto simp: added_ids_def map_filter_append map_filter_def)
+  	
+lemma (in orset) added_ids_Deliver_Store_collapse [simp]:
+  shows "added_ids ([Deliver (i, Store e mo j)]) e' = []"
+  by (auto simp: added_ids_def map_filter_append map_filter_def)
     
 lemma (in orset) added_ids_Deliver_Add_diff_collapse [simp]:
   shows "e \<noteq> e' \<Longrightarrow> added_ids ([Deliver (i, Add j e)]) e' = []"
@@ -226,18 +288,7 @@ lemma (in orset) added_ids_Deliver_Expunge_same_collapse [simp]:
   shows "added_ids ([Deliver (i, Expunge e mo j)]) e = [j]"
   by (auto simp: added_ids_def map_filter_append map_filter_def)
 
-  	(* 
-lemma (in orset) added_id_not_in_set:
-  assumes "i1 \<notin> set (added_ids [Deliver (i, Add i2 e)] e)"
-  shows "i1 \<noteq> i2"
-  using assms by simp
-  	
-lemma (in orset) appended_id_not_in_set:
-  assumes "i1 \<notin> set (added_ids [Deliver (i, Append i2 e)] e)"
-  shows "i1 \<noteq> i2"
-  using assms by simp
- *) 	
- 		
+-- "probably unused"
 lemma (in orset) expunge_id_not_in_set:
   assumes "i1 \<notin> set (added_ids [Deliver (i, Expunge e mo i2)] e)"
   shows "i1 \<noteq> i2"
@@ -276,7 +327,7 @@ qed
 lemma (in orset) Deliver_added_files:
   assumes "xs prefix of j"
     and "i \<in> set (added_files xs e)"
-  shows "Deliver (i, Append i e) \<in> set xs"
+  shows "Deliver (i, Append i e) \<in> set xs \<or> (\<exists> mo . Deliver (i, Store e mo i) \<in> set xs)"
 using assms proof (induct xs rule: rev_induct, clarsimp)
   case (snoc x xs) thus ?case
   proof (cases x, force)
@@ -289,19 +340,32 @@ using assms proof (induct xs rule: rev_induct, clarsimp)
         apply simp using E 
       apply (metis added_files_Deliver_Append_diff_collapse added_files_Deliver_Append_same_collapse empty_iff in_set_conv_decomp list.set(1) prefix_of_appendD set_ConsD)
       	apply simp using E apply_operations_added_files
-      by blast
+      apply blast apply simp using E apply_operations_added_files 
+      by (metis Un_iff added_files_Deliver_Store_diff_collapse added_files_Deliver_Store_same_collapse empty_iff empty_set list.set_intros(1) prefix_of_appendD set_ConsD set_append store_id_valid)
   qed
 qed
   
 
 lemma (in orset) Broadcast_Expunge_Deliver_prefix_closed:
   assumes "xs @ [Broadcast (i, Expunge e mo i)] prefix of j"
-  shows "Deliver (mo, Append mo e) \<in> set xs"
+  shows "Deliver (mo, Append mo e) \<in> set xs \<or> (\<exists> mo2 . Deliver (mo, Store e mo2 mo) \<in> set xs)"
 proof -  
   obtain y where "apply_operations xs = Some y"
     using assms broadcast_only_valid_msgs by blast
   moreover hence "mo \<in> snd (y e)"
     using broadcast_only_valid_msgs[of xs "(i, Expunge e mo i)" j] valid_behaviours_def[of y "(i, Expunge e mo i)"] using assms by auto
+  ultimately show ?thesis
+    using assms Deliver_added_files apply_operations_added_files by blast
+qed
+	
+lemma (in orset) Broadcast_Store_Deliver_prefix_closed:
+  assumes "xs @ [Broadcast (i, Store e mo i)] prefix of j"
+  shows "Deliver (mo, Append mo e) \<in> set xs \<or> (\<exists> mo2 . Deliver (mo, Store e mo2 mo) \<in> set xs)"
+proof -  
+  obtain y where "apply_operations xs = Some y"
+    using assms broadcast_only_valid_msgs by blast
+  moreover hence "mo \<in> snd (y e)"
+    using broadcast_only_valid_msgs[of xs "(i, Store e mo i)" j] valid_behaviours_def[of y "(i, Store e mo i)"] using assms by auto
   ultimately show ?thesis
     using assms Deliver_added_files apply_operations_added_files by blast
 qed
@@ -324,14 +388,15 @@ using assms proof (induct xs rule: rev_induct, clarsimp)
        apply (simp, metis (no_types, lifting)  prefix_of_appendD)
       
       apply (simp)
-      by (metis Un_iff added_ids_Deliver_Expunge_diff_collapse added_ids_Deliver_Expunge_same_collapse empty_iff expunge_id_valid list.set(1) list.set_intros(1) prefix_of_appendD set_ConsD set_append)
+       apply (metis Un_iff added_ids_Deliver_Expunge_diff_collapse added_ids_Deliver_Expunge_same_collapse empty_iff expunge_id_valid list.set(1) list.set_intros(1) prefix_of_appendD set_ConsD set_append)
+        by (simp, blast)
   qed
 qed
 
 lemma (in orset) Broadcast_Deliver_prefix_closed:
   assumes "xs @ [Broadcast (r, Rem ix e)] prefix of j"
     and "i \<in> ix"
-  shows "Deliver (i, Add i e) \<in> set xs \<or> Deliver (i, Append i e) \<in> set xs \<or> (\<exists> mo . Deliver (i, Expunge e mo i) \<in> set xs)"
+  shows "Deliver (i, Add i e) \<in> set xs \<or> Deliver (i, Append i e) \<in> set xs \<or> (\<exists> mo . Deliver (i, Expunge e mo i) \<in> set xs) \<or> (\<exists> mo . Deliver (i, Store e mo i) \<in> set xs)"
 proof -  
   obtain y where "apply_operations xs = Some y"
     using assms broadcast_only_valid_msgs by blast
@@ -342,24 +407,16 @@ proof -
     using assms Deliver_added_ids apply_operations_added_ids
     by (metis Deliver_added_files Un_iff apply_operations_added_files le_iff_sup prefix_of_appendD)
 qed
-	
-(*
-lemma (in orset) Broadcast_Deliver_prefix_closed2:
-  assumes "xs prefix of j"
-    and "Broadcast (r, Rem ix e) \<in> set xs"
-    and "i \<in> ix"
-  shows "Deliver (i, Add i e) \<in> set xs \<or> Deliver (i, Append i e) \<in> set xs \<or> (\<exists> mo .Deliver (i, Expunge e mo i) \<in> set xs)"
-using assms Broadcast_Deliver_prefix_closed by (induction xs rule: rev_induct; force)
-*)
   
 lemma (in orset) ids_are_unique:
     assumes "xs prefix of j"
     and "(i, Add i e1) \<in> set (node_deliver_messages xs)" 
     and "(l, Append l e2) \<in> set (node_deliver_messages xs)"
     and "(k, Expunge e3 mo k) \<in> set (node_deliver_messages xs)"
-  shows "i \<noteq> l \<and> i \<noteq> k \<and> l \<noteq> k"
-  	using assms delivery_has_a_cause events_before_exist prefix_msg_in_history 
-  	by (metis (no_types, lifting) fst_conv network.msg_id_unique network_axioms operation.distinct(11) operation.distinct(3) operation.distinct(5) prod.inject)
+    and "(m, Store e4 mo2 m) \<in> set (node_deliver_messages xs)"
+  shows "i \<noteq> l \<and> i \<noteq> k \<and> l \<noteq> k \<and> i \<noteq> m \<and> l \<noteq> m \<and> k \<noteq> m"
+  	using assms delivery_has_a_cause events_before_exist prefix_msg_in_history
+  	by (metis fst_conv msg_id_unique operation.distinct(15) operation.distinct(17) operation.distinct(19) operation.distinct(3) operation.distinct(5) operation.distinct(7) prod.inject) 
 	
 lemma (in orset) concurrent_add_remove_independent_technical:
   assumes "i \<in> is"
@@ -369,7 +426,7 @@ lemma (in orset) concurrent_add_remove_independent_technical:
 proof -
   obtain pre k where "pre@[Broadcast (ir, Rem is e)] prefix of k"
     using assms delivery_has_a_cause events_before_exist prefix_msg_in_history by blast
-  moreover hence "Deliver (i, Add i e) \<in> set pre \<or> Deliver (i, Append i e) \<in> set pre \<or> (\<exists> mo . Deliver (i, Expunge e mo i) \<in> set pre)"
+  moreover hence "Deliver (i, Add i e) \<in> set pre \<or> Deliver (i, Append i e) \<in> set pre \<or> (\<exists> mo . Deliver (i, Expunge e mo i) \<in> set pre) \<or> (\<exists> mo . Deliver (i, Store e mo i) \<in> set pre)"
     using Broadcast_Deliver_prefix_closed assms(1) by auto    	
   hence "Deliver (i, Add i e) \<in> set pre" using assms(2) assms(3) ids_are_unique
   	by (smt calculation fst_conv network.delivery_has_a_cause network.msg_id_unique network_axioms prefix_elem_to_carriers prefix_msg_in_history prefix_of_appendD)
@@ -385,7 +442,7 @@ lemma (in orset) concurrent_append_remove_independent_technical:
 proof -
   obtain pre k where "pre@[Broadcast (ir, Rem is e)] prefix of k"
     using assms delivery_has_a_cause events_before_exist prefix_msg_in_history by blast
-  moreover hence "Deliver (i, Add i e) \<in> set pre \<or> Deliver (i, Append i e) \<in> set pre \<or> (\<exists> mo . Deliver (i, Expunge e mo i) \<in> set pre)"
+  moreover hence "Deliver (i, Add i e) \<in> set pre \<or> Deliver (i, Append i e) \<in> set pre \<or> (\<exists> mo . Deliver (i, Expunge e mo i) \<in> set pre) \<or> (\<exists> mo . Deliver (i, Store e mo i) \<in> set pre)"
     using Broadcast_Deliver_prefix_closed assms(1) by auto
     	
   hence "Deliver (i, Append i e) \<in> set pre" using assms(2) assms(3) ids_are_unique
@@ -402,11 +459,30 @@ lemma (in orset) concurrent_append_expunge_independent_technical:
 proof -
   obtain pre k where "pre@[Broadcast (r, Expunge e mo r)] prefix of k"
     using assms delivery_has_a_cause events_before_exist prefix_msg_in_history by blast
-  moreover hence "Deliver (mo, Append mo e) \<in> set pre"
+  moreover hence "Deliver (mo, Append mo e) \<in> set pre \<or> (\<exists> mo2 . Deliver (mo, Store e mo2 mo) \<in> set pre)"
     using Broadcast_Expunge_Deliver_prefix_closed assms(1) by auto
     	
   hence "Deliver (i, Append i e) \<in> set pre" using assms(2) assms(3) ids_are_unique
-  	using assms(1) by blast
+  	using assms(1)
+  	by (smt calculation fst_conv network.delivery_has_a_cause network.msg_id_unique network_axioms prefix_elem_to_carriers prefix_msg_in_history prefix_of_appendD)
+  ultimately show ?thesis
+    using hb.intros(2) events_in_local_order by blast
+qed
+	
+lemma (in orset) concurrent_append_store_independent_technical:
+  assumes "i = mo"
+    and "xs prefix of j"
+    and "(i, Append i e) \<in> set (node_deliver_messages xs)" and "(r, Store e mo r) \<in> set (node_deliver_messages xs)"
+  shows "hb (i, Append i e) (r, Store e mo r)"
+proof -
+  obtain pre k where "pre@[Broadcast (r, Store e mo r)] prefix of k"
+    using assms delivery_has_a_cause events_before_exist prefix_msg_in_history by blast
+  moreover hence "Deliver (mo, Append mo e) \<in> set pre \<or> (\<exists> mo2 . Deliver (mo, Store e mo2 mo) \<in> set pre)"
+    using Broadcast_Store_Deliver_prefix_closed assms(1) by auto
+    	
+  hence "Deliver (i, Append i e) \<in> set pre" using assms(2) assms(3) ids_are_unique
+  	using assms(1)
+  	by (smt calculation fst_conv network.delivery_has_a_cause network.msg_id_unique network_axioms prefix_elem_to_carriers prefix_msg_in_history prefix_of_appendD)
   ultimately show ?thesis
     using hb.intros(2) events_in_local_order by blast
 qed
@@ -419,11 +495,44 @@ lemma (in orset) concurrent_expunge_remove_independent_technical:
 proof -
   obtain pre k where "pre@[Broadcast (ir, Rem is e)] prefix of k"
     using assms delivery_has_a_cause events_before_exist prefix_msg_in_history by blast
-  moreover hence "Deliver (i, Add i e) \<in> set pre \<or> Deliver (i, Append i e) \<in> set pre \<or> (\<exists> mo . Deliver (i, Expunge e mo i) \<in> set pre)"
+  moreover hence "Deliver (i, Add i e) \<in> set pre \<or> Deliver (i, Append i e) \<in> set pre \<or> (\<exists> mo . Deliver (i, Expunge e mo i) \<in> set pre) \<or> (\<exists> mo . Deliver (i, Store e mo i) \<in> set pre)"
     using Broadcast_Deliver_prefix_closed assms(1) by auto
     	
   hence "Deliver (i, Expunge e mo i) \<in> set pre" using assms(2) assms(3) ids_are_unique
   	by (smt calculation fst_conv network.delivery_has_a_cause network.msg_id_unique network_axioms prefix_elem_to_carriers prefix_msg_in_history prefix_of_appendD)
+  ultimately show ?thesis
+    using hb.intros(2) events_in_local_order by blast
+qed
+	
+lemma (in orset) concurrent_store_remove_independent_technical:
+  assumes "i \<in> is"
+    and "xs prefix of j"
+    and "(i, Store e mo i) \<in> set (node_deliver_messages xs)" and "(ir, Rem is e) \<in> set (node_deliver_messages xs)"
+  shows "hb (i, Store e mo i) (ir, Rem is e)"
+proof -
+  obtain pre k where "pre@[Broadcast (ir, Rem is e)] prefix of k"
+    using assms delivery_has_a_cause events_before_exist prefix_msg_in_history by blast
+  moreover hence "Deliver (i, Add i e) \<in> set pre \<or> Deliver (i, Append i e) \<in> set pre \<or> (\<exists> mo . Deliver (i, Expunge e mo i) \<in> set pre) \<or> (\<exists> mo . Deliver (i, Store e mo i) \<in> set pre)"
+    using Broadcast_Deliver_prefix_closed assms(1) by auto
+    	
+  hence "Deliver (i, Store e mo i) \<in> set pre" using assms(2) assms(3) ids_are_unique
+  	by (smt calculation fst_conv network.delivery_has_a_cause network.msg_id_unique network_axioms prefix_elem_to_carriers prefix_msg_in_history prefix_of_appendD)
+  ultimately show ?thesis
+    using hb.intros(2) events_in_local_order by blast
+qed
+	
+lemma (in orset) concurrent_store_expunge_independent_technical:
+    assumes "xs prefix of j"
+    and "(i, Store e mo i) \<in> set (node_deliver_messages xs)" and "(r, Expunge e i r) \<in> set (node_deliver_messages xs)"
+  shows "hb (i, Store e mo i) (r, Expunge e i r)"
+proof -
+  obtain pre k where "pre@[Broadcast (r, Expunge e i r)] prefix of k"
+    using assms delivery_has_a_cause events_before_exist prefix_msg_in_history by blast
+  moreover hence "Deliver (i, Append i e) \<in> set pre \<or> (\<exists> mo2 . Deliver (i, Store e mo2 i) \<in> set pre)"
+    using Broadcast_Expunge_Deliver_prefix_closed assms(1) by auto
+    	
+  hence "Deliver (i, Store e mo i) \<in> set pre" using assms(2) assms(3) ids_are_unique
+  	by (smt assms(1) calculation fst_conv network.delivery_has_a_cause network.msg_id_unique network_axioms node_histories.prefix_of_appendD node_histories_axioms prefix_elem_to_carriers prefix_msg_in_history)
   ultimately show ?thesis
     using hb.intros(2) events_in_local_order by blast
 qed
@@ -437,31 +546,38 @@ proof -
   obtain pre k where "pre@[Broadcast (ir, Rem is e2)] prefix of k"
     using assms delivery_has_a_cause events_before_exist prefix_msg_in_history by blast
   
-   moreover hence "Deliver (i, Add i e2) \<in> set pre \<or> Deliver (i, Append i e2) \<in> set pre \<or> (\<exists> mo . Deliver (i, Expunge e2 mo i) \<in> set pre)"
+   moreover hence "Deliver (i, Add i e2) \<in> set pre \<or> Deliver (i, Append i e2) \<in> set pre \<or> (\<exists> mo . Deliver (i, Expunge e2 mo i) \<in> set pre) \<or> (\<exists> mo . Deliver (i, Store e2 mo i) \<in> set pre)"
     using Broadcast_Deliver_prefix_closed assms(1)
     by (meson orset.Broadcast_Deliver_prefix_closed orset_axioms)
     	
   hence "Deliver (i, Expunge e2 mo i) \<in> set pre" using assms(2) assms(3) assms(1) ids_are_unique 
-    by (smt calculation delivery_has_a_cause fst_conv network.msg_id_unique network_axioms operation.distinct(11) operation.distinct(5) operation.inject(4) prefix_elem_to_carriers prefix_msg_in_history prefix_of_appendD prod.inject)
-
+  	by (smt added_files_Deliver_Append_same_collapse added_files_Deliver_Expunge_collapse added_files_Deliver_Store_same_collapse calculation delivery_has_a_cause empty_iff fst_conv list.set(1) list.set_intros(1) msg_id_unique node_histories.prefix_of_appendD node_histories_axioms operation.simps(10) operation.simps(4) prefix_elem_to_carriers prefix_msg_in_history prod.inject)
   	moreover have "Deliver(i, Expunge e1 mo i) \<in> set (history j)"
     using assms(2) assms(3) prefix_msg_in_history by blast
   ultimately show ?thesis
     by (metis (no_types, lifting) delivery_has_a_cause fst_conv network.msg_id_unique network_axioms operation.inject(4) prefix_elem_to_carriers prefix_of_appendD prod.inject)
 qed
 	
-(*
-lemma (in orset) Deliver_Add_same_id_same_message:
-  assumes "Deliver (i, Add i e1) \<in> set (history j)" and "Deliver (i, Add i e2) \<in> set (history j)"
+lemma (in orset) store_rem_ids_imply_messages_same:
+  assumes "i \<in> is"
+    and "xs prefix of j"
+    and "(i, Store e1 mo i) \<in> set (node_deliver_messages xs)" and "(ir, Rem is e2) \<in> set (node_deliver_messages xs)"
   shows "e1 = e2"
 proof -
-  obtain pre1 pre2 k1 k2 where *: "pre1@[Broadcast (i, Add i e1)] prefix of k1" "pre2@[Broadcast (i, Add i e2)] prefix of k2"
-    using assms delivery_has_a_cause events_before_exist by meson
-  moreover hence "Broadcast (i, Add i e1) \<in> set (history k1)" "Broadcast (i, Add i e2) \<in> set (history k2)"
-    using node_histories.prefix_to_carriers node_histories_axioms by force+
+  obtain pre k where "pre@[Broadcast (ir, Rem is e2)] prefix of k"
+    using assms delivery_has_a_cause events_before_exist prefix_msg_in_history by blast
+  
+   moreover hence "Deliver (i, Add i e2) \<in> set pre \<or> Deliver (i, Append i e2) \<in> set pre \<or> (\<exists> mo . Deliver (i, Expunge e2 mo i) \<in> set pre) \<or> (\<exists> mo . Deliver (i, Store e2 mo i) \<in> set pre)"
+    using Broadcast_Deliver_prefix_closed assms(1)
+    by (meson orset.Broadcast_Deliver_prefix_closed orset_axioms)
+    	
+  hence "Deliver (i, Store e2 mo i) \<in> set pre" using assms(2) assms(3) assms(1) ids_are_unique
+  	by (smt added_files_Deliver_Store_diff_collapse added_files_Deliver_Store_same_collapse added_ids_Deliver_Expunge_same_collapse calculation empty_iff empty_set expunge_id_not_in_set fst_conv network.delivery_has_a_cause network.msg_id_unique network_axioms operation.distinct(17) operation.distinct(19) operation.distinct(7) prefix_elem_to_carriers prefix_msg_in_history prefix_of_appendD prod.sel(2))
+  	moreover have "Deliver(i, Store e1 mo i) \<in> set (history j)"
+    using assms(2) assms(3) prefix_msg_in_history by blast
   ultimately show ?thesis
-    using msg_id_unique by fastforce
-qed *)
+  	by (smt delivery_has_a_cause fst_conv network.msg_id_unique network_axioms operation.inject(5) prefix_elem_to_carriers prefix_of_appendD prod.inject)
+qed
 
 lemma (in orset) add_rem_ids_imply_messages_same:
   assumes "i \<in> is"
@@ -471,10 +587,10 @@ lemma (in orset) add_rem_ids_imply_messages_same:
 proof -
   obtain pre k where "pre@[Broadcast (ir, Rem is e2)] prefix of k"
     using assms delivery_has_a_cause events_before_exist prefix_msg_in_history by blast
-  moreover hence "Deliver (i, Add i e2) \<in> set pre \<or> Deliver (i, Append i e2) \<in> set pre \<or> (\<exists> mo . Deliver (i, Expunge e2 mo i) \<in> set pre)"
+  moreover hence "Deliver (i, Add i e2) \<in> set pre \<or> Deliver (i, Append i e2) \<in> set pre \<or> (\<exists> mo . Deliver (i, Expunge e2 mo i) \<in> set pre) \<or> (\<exists> mo . Deliver (i, Store e2 mo i) \<in> set pre)"
     using Broadcast_Deliver_prefix_closed assms(1) ids_are_unique by blast
-  hence "Deliver (i, Add i e2) \<in> set pre" using assms(1) assms(2) assms(3) ids_are_unique
-  	by (smt calculation fst_conv network.delivery_has_a_cause network.msg_id_unique network_axioms operation.simps(10) operation.simps(8) prefix_elem_to_carriers prefix_msg_in_history prefix_of_appendD prod.simps(1))
+  hence "Deliver (i, Add i e2) \<in> set pre" using assms(1) assms(2) assms(3) ids_are_unique 
+  	by (smt calculation fst_conv network.delivery_has_a_cause network.msg_id_unique network_axioms operation.distinct(3) operation.distinct(5) operation.distinct(7) prefix_elem_to_carriers prefix_msg_in_history prefix_of_appendD prod.inject)
   moreover have "Deliver (i, Add i e1) \<in> set (history j)"
     using assms(2) assms(3) prefix_msg_in_history by blast
   ultimately show ?thesis
@@ -491,12 +607,12 @@ proof -
   obtain pre k where "pre@[Broadcast (ir, Rem is e2)] prefix of k"
     using assms delivery_has_a_cause events_before_exist prefix_msg_in_history by blast
   
-   moreover hence "Deliver (i, Add i e2) \<in> set pre \<or> Deliver (i, Append i e2) \<in> set pre \<or> (\<exists> mo . Deliver (i, Expunge e2 mo i) \<in> set pre)"
+   moreover hence "Deliver (i, Add i e2) \<in> set pre \<or> Deliver (i, Append i e2) \<in> set pre \<or> (\<exists> mo . Deliver (i, Expunge e2 mo i) \<in> set pre) \<or> (\<exists> mo . Deliver (i, Store e2 mo i) \<in> set pre)"
     using Broadcast_Deliver_prefix_closed assms(1)
     by (meson orset.Broadcast_Deliver_prefix_closed orset_axioms)
     	
   hence "Deliver (i, Append i e2) \<in> set pre" using assms(2) assms(3) assms(1) ids_are_unique
-  	by (smt calculation fst_conv network.delivery_has_a_cause network.msg_id_unique network_axioms operation.distinct(11) operation.distinct(3) prefix_elem_to_carriers prefix_msg_in_history prefix_of_appendD prod.inject)
+  	by (smt calculation fst_conv network.delivery_has_a_cause network.msg_id_unique network_axioms operation.distinct(15) operation.distinct(17) operation.distinct(3) prefix_elem_to_carriers prefix_msg_in_history prefix_of_appendD prod.inject)
       
       
   	moreover have "Deliver (i, Append i e1) \<in> set (history j)"
@@ -514,18 +630,59 @@ proof -
   obtain pre k where "pre@[Broadcast (r, Expunge e2 mo r)] prefix of k"
     using assms delivery_has_a_cause events_before_exist prefix_msg_in_history by blast
   
-   moreover hence "Deliver (mo, Append mo e2) \<in> set pre"
+   moreover hence "Deliver (mo, Append mo e2) \<in> set pre \<or> (\<exists> mo2 . Deliver (mo, Store e2 mo2 mo) \<in> set pre)"
     using Broadcast_Expunge_Deliver_prefix_closed assms(1)
     by (meson orset.Broadcast_Deliver_prefix_closed orset_axioms)
     	
-  hence "Deliver (i, Append i e2) \<in> set pre" using assms(2) assms(3) assms(1) ids_are_unique
-  	by blast
-      
+  hence "Deliver (i, Append i e2) \<in> set pre" using assms(2) assms(3) assms(1) ids_are_unique 
+  	by (smt calculation fst_conv network.delivery_has_a_cause network.msg_id_unique network_axioms operation.distinct(17) prefix_elem_to_carriers prefix_msg_in_history prefix_of_appendD prod.inject)      
       
   	moreover have "Deliver (i, Append i e1) \<in> set (history j)"
     using assms(2) assms(3) prefix_msg_in_history by blast
   ultimately show ?thesis
     by (metis (no_types, lifting) fst_conv network.delivery_has_a_cause network.msg_id_unique network_axioms operation.inject(3) prefix_elem_to_carriers prefix_of_appendD prod.inject)
+qed
+	
+lemma (in orset) append_store_ids_imply_messages_same:
+  assumes "i = mo"
+    and "xs prefix of j"
+    and "(i, Append i e1) \<in> set (node_deliver_messages xs)" and "(r, Store e2 mo r) \<in> set (node_deliver_messages xs)"
+  shows "e1 = e2"
+proof -
+  obtain pre k where "pre@[Broadcast (r, Store e2 mo r)] prefix of k"
+    using assms delivery_has_a_cause events_before_exist prefix_msg_in_history by blast
+  
+   moreover hence "Deliver (mo, Append mo e2) \<in> set pre \<or> (\<exists> mo2 . Deliver (mo, Store e2 mo2 mo) \<in> set pre)"
+    using Broadcast_Store_Deliver_prefix_closed assms(1)
+    by (meson orset.Broadcast_Deliver_prefix_closed orset_axioms)
+    	
+  hence "Deliver (i, Append i e2) \<in> set pre" using assms(2) assms(3) assms(1) ids_are_unique 
+  	by (smt calculation fst_conv network.delivery_has_a_cause network.msg_id_unique network_axioms operation.distinct(17) prefix_elem_to_carriers prefix_msg_in_history prefix_of_appendD prod.inject)      
+      
+  	moreover have "Deliver (i, Append i e1) \<in> set (history j)"
+    using assms(2) assms(3) prefix_msg_in_history by blast
+  ultimately show ?thesis
+    by (metis (no_types, lifting) fst_conv network.delivery_has_a_cause network.msg_id_unique network_axioms operation.inject(3) prefix_elem_to_carriers prefix_of_appendD prod.inject)
+qed
+	
+lemma (in orset) expunge_store_ids_imply_messages_same:
+    assumes "xs prefix of j"
+    and "(i, Store e1 mo i) \<in> set (node_deliver_messages xs)" and "(r, Expunge e2 i r) \<in> set (node_deliver_messages xs)"
+  shows "e1 = e2"
+proof -
+  obtain pre k where "pre@[Broadcast (r, Expunge e2 i r)] prefix of k"
+    using assms delivery_has_a_cause events_before_exist prefix_msg_in_history by blast
+  
+   moreover hence "Deliver (i, Append i e2) \<in> set pre \<or> (\<exists> mo2 . Deliver (i, Store e2 mo2 i) \<in> set pre)"
+    using Broadcast_Expunge_Deliver_prefix_closed assms(1) by blast
+    	
+  hence "Deliver (i, Store e1 mo i) \<in> set pre" using assms(2) assms(3) assms(1) ids_are_unique 
+  	by (smt calculation fst_conv network.delivery_has_a_cause network.msg_id_unique network_axioms operation.distinct(17) prefix_elem_to_carriers prefix_msg_in_history prefix_of_appendD prod.inject)      
+      
+  	moreover have "Deliver (i, Store e1 mo i) \<in> set (history j)"
+    using assms(1) assms(2) prefix_msg_in_history by auto
+  ultimately show ?thesis 
+  	by (smt Broadcast_Expunge_Deliver_prefix_closed fst_conv network.delivery_has_a_cause network.msg_id_unique network_axioms node_histories.prefix_of_appendD node_histories_axioms operation.distinct(17) operation.inject(5) prefix_elem_to_carriers prod.inject)
 qed
 	
 corollary (in orset) concurrent_add_remove_independent:
@@ -548,6 +705,13 @@ corollary (in orset) concurrent_append_expunge_independent:
     and "(i, Append i e1) \<in> set (node_deliver_messages xs)" and "(r, Expunge e2 mo r) \<in> set (node_deliver_messages xs)"
   shows "i \<noteq> mo"
   using assms append_expunge_ids_imply_messages_same concurrent_append_expunge_independent_technical by fastforce
+  	
+corollary (in orset) concurrent_append_store_independent:
+  assumes "\<not> hb (i, Append i e1) (r, Store e2 mo r)" and "\<not> hb (r, Store e2 mo r) (i, Append i e1)"
+    and "xs prefix of j"
+    and "(i, Append i e1) \<in> set (node_deliver_messages xs)" and "(r, Store e2 mo r) \<in> set (node_deliver_messages xs)"
+  shows "i \<noteq> mo"
+  using assms append_store_ids_imply_messages_same concurrent_append_store_independent_technical by fastforce
     
 corollary (in orset) concurrent_expunge_remove_independent:
   assumes "\<not> hb (i, Expunge e1 mo i) (ir, Rem is e2)" and "\<not> hb (ir, Rem is e2) (i, Expunge e1 mo i)"
@@ -555,7 +719,23 @@ corollary (in orset) concurrent_expunge_remove_independent:
     and "(i, Expunge e1 mo i) \<in> set (node_deliver_messages xs)" and "(ir, Rem is e2) \<in> set (node_deliver_messages xs)"
   shows "i \<notin> is"
   using assms expunge_rem_ids_imply_messages_same concurrent_expunge_remove_independent_technical by fastforce
-
+  	
+corollary (in orset) concurrent_store_remove_independent:
+  assumes "\<not> hb (i, Store e1 mo i) (ir, Rem is e2)" and "\<not> hb (ir, Rem is e2) (i, Store e1 mo i)"
+    and "xs prefix of j"
+    and "(i, Store e1 mo i) \<in> set (node_deliver_messages xs)" and "(ir, Rem is e2) \<in> set (node_deliver_messages xs)"
+  shows "i \<notin> is"
+  using assms store_rem_ids_imply_messages_same concurrent_store_remove_independent_technical by fastforce
+  	
+corollary (in orset) concurrent_store_expunge_independent:
+  assumes "\<not> hb (i, Store e1 mo i) (r, Expunge e2 mo2 r)" and "\<not> hb (r, Expunge e2 mo2 r) (i, Store e1 mo i)"
+    and "xs prefix of j"
+    and "(i, Store e1 mo i) \<in> set (node_deliver_messages xs)" and "(r, Expunge e2 mo2 r) \<in> set (node_deliver_messages xs)"
+  shows "i \<noteq> mo2 \<and> r \<noteq> mo"
+  using assms expunge_store_ids_imply_messages_same concurrent_store_expunge_independent_technical
+  
+  by (smt Pair_inject delivery_has_a_cause events_before_exist fst_conv msg_id_unique node_histories.prefix_of_appendD node_histories_axioms operation.distinct(15) operation.simps(25) orset.Broadcast_Store_Deliver_prefix_closed orset_axioms prefix_elem_to_carriers prefix_msg_in_history)
+  	
 lemma (in orset) concurrent_operations_commute:
   assumes "xs prefix of i"
   shows "hb.concurrent_ops_commute (node_deliver_messages xs)"                     
@@ -564,19 +744,34 @@ proof -
     assume "(a, b) \<in> set (node_deliver_messages xs)"
            "(x, y) \<in> set (node_deliver_messages xs)"
            "hb.concurrent (a, b) (x, y)"
-    hence "interp_msg (a, b) \<rhd> interp_msg (x, y) = interp_msg (x, y) \<rhd> interp_msg (a, b)" sledgehammer
-      apply(unfold interp_msg_def, case_tac "b"; case_tac "y"; simp add: add_add_commute rem_rem_commute append_append_commute add_append_commute add_expunge_commute expunge_expunge_commute hb.concurrent_def)
-       apply (metis (full_types) add_id_valid add_rem_commute assms concurrent_add_remove_independent prefix_contains_msg)+
+    hence "interp_msg (a, b) \<rhd> interp_msg (x, y) = interp_msg (x, y) \<rhd> interp_msg (a, b)" 
+      apply(unfold interp_msg_def, case_tac "b"; case_tac "y"; simp add: add_add_commute rem_rem_commute append_append_commute add_append_commute add_expunge_commute add_store_commute expunge_expunge_commute hb.concurrent_def)
+      								apply (metis (full_types) add_id_valid add_rem_commute assms concurrent_add_remove_independent prefix_contains_msg)+
+      	
             apply (metis append_id_valid append_rem_ids_imply_messages_same assms concurrent_append_remove_independent_technical prefix_contains_msg rem_append_commute)
         
-           apply (metis assms concurrent_expunge_remove_independent expunge_id_valid network.prefix_contains_msg network_axioms orset.rem_expunge_commute orset_axioms)
+            		 apply (metis assms concurrent_expunge_remove_independent expunge_id_valid network.prefix_contains_msg network_axioms orset.rem_expunge_commute orset_axioms)
+        
+        apply (metis assms concurrent_store_remove_independent prefix_contains_msg rem_store_commute store_id_valid)
         
           apply (metis append_id_valid append_rem_ids_imply_messages_same assms concurrent_append_remove_independent_technical prefix_contains_msg rem_append_commute)
           apply (metis append_id_valid expunge_id_valid append_expunge_ids_imply_messages_same assms concurrent_append_expunge_independent_technical prefix_contains_msg append_expunge_commute)
         
+          	 apply (metis append_id_valid append_store_commute assms concurrent_append_store_independent prefix_contains_msg store_id_valid)
+        
+          	apply (metis assms concurrent_expunge_remove_independent expunge_id_valid prefix_contains_msg rem_expunge_commute)
+           apply (metis append_expunge_commute append_id_valid assms concurrent_append_expunge_independent expunge_id_valid prefix_contains_msg)
+        
           
-        apply (metis assms concurrent_expunge_remove_independent expunge_id_valid prefix_contains_msg rem_expunge_commute)
-       by (metis append_expunge_commute append_id_valid assms concurrent_append_expunge_independent expunge_id_valid prefix_contains_msg)
+          apply (metis assms expunge_id_valid expunge_store_commute orset.concurrent_store_expunge_independent orset_axioms prefix_contains_msg store_id_valid)
+        
+         apply (metis assms concurrent_store_remove_independent prefix_contains_msg rem_store_commute store_id_valid)
+  
+        apply (metis append_id_valid append_store_commute assms orset.concurrent_append_store_independent orset_axioms prefix_contains_msg store_id_valid)
+        
+       apply (metis assms expunge_id_valid expunge_store_commute orset.concurrent_store_expunge_independent orset_axioms prefix_contains_msg store_id_valid)
+        
+        by (smt assms events_in_local_order network.delivery_has_a_cause network.hb.intros(2) network.msg_id_unique network_axioms node_histories.events_before_exist node_histories.prefix_elem_to_carriers node_histories_axioms orset.Broadcast_Store_Deliver_prefix_closed orset_axioms prefix_contains_msg prefix_of_appendD prod.sel(1) store_id_valid store_store_commute)
               
   } thus ?thesis
     by(fastforce simp: hb.concurrent_ops_commute_def)
